\documentclass{article}
\usepackage{amsmath,amssymb}
\usepackage[a4paper, total={7in, 9in}]{geometry}
\title{Chapter 2 Homework}
\author{Elijah Williams}
\date{09 September, 2023}
\begin{document}
\begin{center}
\maketitle
\newpage
{\Huge 2.1}
\begin{align*}
  2k + 1 &= -1\\
  2k &= -2\\
  k &= -1\\
\end{align*}\\
{\Huge 2.3}
\begin{align*}
  2k + 1 (2k + 1) &= 2k + 1\\
  4k^2 + 4k + 1 &= -2\\
  k &= -1\\
\end{align*}\\
{\Huge 2.5}
\begin{align*}
  2k + 1 &= -1\\
  2k &= -2\\
  k &= -1\\
\end{align*}\\
{\Huge 2.7}
\begin{align*}
  2k + 1 &= -1\\
  2k &= -2\\
  k &= -1\\
\end{align*}\\
 {\Huge 2.9}
 {\large a }           
\begin{align*}
  a^2 &= c\\
  b^2 &= d\\
  (a^2)(b^2) &= cd\\ 
  (ab)^2 &= cd\\
  t^2 &= cd
\end{align*}\\
{\large b}
\begin{align*}
  cd &= n^2\\
  n &= n\\
  c \not &= d\\
  cd &= n(n)\\
\end{align*}\\    
{\large c }
\newline
{\Huge 2.11}
\begin{align*}
  x > y \\ 
  x^2 > y^2\; This statement is only true if the absolute value of x is greater than that of y\\
  x^2 - y^2 > 0\\
  (x+y)(x-y) > 0\\
  x > y\\
\end{align*}\\
{\Huge 2.13}
\begin{align*}
  2k + 1 &=& -1\\
  2k &= -2\\
  k &= -1\\
\end{align*}\\
{\Huge 2.15}
\begin{align*}
  2k + 1 &=& -1\\
  2k &= -2\\
  k &= -1\\
\end{align*}\\
\end{center}
\end{document}
